# Week 3 - Lecture 6 - September 21, 2017
## Examples
### 3.12 Consider the following grammar:
1. `<S> -> a <S> c <B> | <A> | b`
2. `<A> -> c <A> | c`
3. `<B> -> d | <A>`

### Which of the following sentences are generated by this grammar?
a. `abcd` - √
  - 1a.  `a <S> c <B>`
  - 2c. `abc <B>`
  - 3a. `abcd`

b. `acccbd` - X // You cannot produce a `b` following `c`
  - 1a. `a <S> c <B>`
  - 2a. `ac <A> c <B>`
  - 2b. `accc <B>` // Dead end; can't produce a `b` from <B>

c. `acccbcc` - X

d. `acd` - X // Requires at least 2 `c`'s

e. `accc` - √
